src/PushButtonSynthesis/UnsaturatedSolinas.v
@@ -104,11 +104,8 @@ Section __.
           {widen_carry : widen_carry_opt}
           {widen_bytes : widen_bytes_opt}
           {tight_upperbound_fraction : tight_upperbound_fraction_opt}
-          {assembly_calling_registers : assembly_calling_registers_opt}
-          {assembly_stack_size : assembly_stack_size_opt}
+          {assembly_conventions : assembly_conventions_opt}
           {error_on_unused_assembly_functions : error_on_unused_assembly_functions_opt}
-          {assembly_output_first : assembly_output_first_opt}
-          {assembly_argument_registers_left_to_right : assembly_argument_registers_left_to_right_opt}
           (n : nat)
           (s : Z)
           (c : list (Z * Z))
